Prove and use Commit in transfer_yield
Spec still doesn't say anything particularly interesting about how the
ledger was transformed (eg, giving transactions IDs), but it does
modify the state correctly.

The proofs are also cleaned up a bit to use more lemmas, and use them
via automation.

src/EventCSL.v
@@ -64,7 +64,7 @@ Section EventCSL.
       step m s (Yield rx) m' s (rx tt)
   | StepCommit : forall m s up rx,
       StateR s (up s) ->
-      StateI s m ->
+      StateI (up s) m ->
       step m s (Commit up rx) m (up s) (rx tt).
 
   Hint Constructors step.
@@ -178,7 +178,7 @@ Section EventCSL.
   Qed.
 
   Theorem commit_failure'_inv : forall m s up rx,
-    (~StateI s m) ->
+    (~StateI (up s) m) ->
     (~ exists m' s' p', step m s (Commit up rx) m' s' p').
   Proof.
     not_sidecondition_fail.
@@ -230,7 +230,7 @@ Section EventCSL.
       destruct (InvDec m);
       destruct (StateI_dec s m); eauto.
     - case_eq (StateR_dec s (up s));
-      case_eq (StateI_dec s m).
+      case_eq (StateI_dec (up s) m).
       rx_specialize m (up s).
       all: eauto 15.
     - eauto.
@@ -363,6 +363,21 @@ Section EventCSL.
     - contradiction H0; eauto.
   Qed.
 
+  Theorem commit_ok : forall up,
+    {{ F s0,
+     | PRE s: F * [[ s = s0 ]] * [[ StateR s0 (up s0) ]] * [[ F =p=> StateI (up s0) ]]
+     | POST s': RET:_ F * [[ s' = up s0 ]]
+    }} Commit up.
+  Proof.
+    unfold valid at 1; intros.
+    destruct_lift H.
+    ind_exec.
+    - prove_rx.
+      simpl.
+      eapply pimpl_apply; [cancel | auto].
+    - contradiction H0; eauto 10.
+  Qed.
+
   Theorem pimpl_ok : forall pre pre' p,
       valid pre p ->
       (forall d s, pre' d s =p=> pre d s) ->
@@ -437,6 +452,7 @@ Arguments Yield {T} {S} rx.
 Hint Extern 1 (valid _ _ _ _ (progseq (Read _) _)) => apply read_ok : prog.
 Hint Extern 1 (valid _ _ _ _ (progseq (Write _ _) _)) => apply write_ok : prog.
 Hint Extern 1 (valid _ _ _ _ (progseq (Yield) _)) => apply yield_ok : prog.
+Hint Extern 1 (valid _ _ _ _ (progseq (Commit _) _)) => apply commit_ok : prog.
 
 Section Bank.
   Definition acct1 : addr := $0.
@@ -478,13 +494,28 @@ Section Bank.
   Definition bankI ledger bal1 bal2 :=
     balances ledger = (bal1, bal2).
 
-  Definition bankS : transitions State :=
-    Build_transitions bankR (fun ledger m => forall bal1 bal2,
-                                 m acct1 = Some bal1 ->
-                                 m acct2 = Some bal2 ->
-                                 bankI ledger #bal1 #bal2).
+  Definition bankPred ledger : @pred addr (@weq addrlen) valu :=
+    (fun m => forall bal1 bal2,
+         m acct1 = Some bal1 ->
+         m acct2 = Some bal2 ->
+         bankI ledger #bal1 #bal2).
 
-  Local Hint Unfold rep inv_rep Inv State bankI : prog.
+  Definition bankS : transitions State :=
+    Build_transitions bankR bankPred.
+
+  Local Hint Unfold rep inv_rep Inv State bankR bankI : prog.
+
+  Definition transfer {T S} rx : prog T S :=
+    bal1 <- Read acct1;
+    bal2 <- Read acct2;
+    Write acct1 (bal1 ^- $1);;
+          Write acct2 (bal2 ^+ $1);;
+          rx tt.
+
+  (* an update function that adds an entry to the ledger for transfer *)
+  Definition record_transfer ledger : State := (from1 1) :: ledger.
+
+  Hint Unfold record_transfer : prog.
 
   Lemma max_balance : forall bal1 bal2,
     (exists F, F * inv_rep bal1 bal2) =p=>
@@ -498,21 +529,82 @@ Section Bank.
     pred_apply; cancel.
   Qed.
 
-  Definition transfer {T S} rx : prog T S :=
-    bal1 <- Read acct1;
-    bal2 <- Read acct2;
-    Write acct1 (bal1 ^- $1);;
-    Write acct2 (bal2 ^+ $1);;
-    rx tt.
+  Lemma pair_eq : forall T S (a1 b1:T) (a2 b2:S),
+      a1 = b1 /\ a2 = b2 <->
+      (a1, a2) = (b1, b2).
+  Proof.
+    intros.
+    intuition; try inversion H; subst; auto.
+  Qed.
 
-  (* an update function that adds an entry to the ledger for transfer *)
-  Definition record_transfer ledger : State := (from1 1) :: ledger.
+  Hint Resolve -> gt0_wneq0.
+
+  Lemma inv_transfer_stable : forall (bal1 bal2 : valu),
+      #bal1 + #bal2 = 100 ->
+      #bal1 > 0 ->
+      # (bal1 ^- $1) + # (bal2 ^+ $1) = 100.
+  Proof.
+    intros.
+    rewrite wordToNat_minus_one by auto.
+    erewrite wordToNat_plusone.
+    omega.
+    apply lt_wlt.
+    instantiate (1 := $101).
+    simpl; omega.
+  Qed.
+
+  Lemma record_correct : forall (bal1 bal2:valu),
+      #bal1 > 0 ->
+      #bal1 + #bal2 = 100 ->
+      (# (bal1) - 1, # (bal2) + 1) =
+      (# (bal1 ^- $ (1)), # (bal2 ^+ $ (1))).
+  Proof.
+    intros.
+    rewrite wordToNat_minus_one by auto.
+    erewrite wordToNat_plusone.
+    apply pair_eq; omega.
+    apply lt_wlt.
+    instantiate (1 := $101).
+    simpl; omega.
+  Qed.
+
+  Hint Resolve record_correct.
+
+  Ltac combine_opt_eq :=
+    match goal with
+    | [ H1 : ?m ?acct = ?rhs, H2 : ?m ?acct = _  |- _ ] =>
+      rewrite H1 in H2; inversion H2;
+      match rhs with
+      | Some ?obj => subst obj
+      end
+    end.
+
+  Lemma bank_invariant_transfer : forall F s bal1 bal2,
+      #bal1 > 0 ->
+      #bal1 + #bal2 = 100 ->
+      balances s = (#bal1, #bal2) ->
+      acct2 |-> (bal2 ^+ $ (1)) * acct1 |-> (bal1 ^- $ (1)) * F =p=>
+  bankPred (from1 1 :: s).
+  Proof.
+    unfold bankPred.
+    autounfold with prog.
+    intros.
+    intro m; intros.
+    assert (m acct1 = Some (bal1 ^- $1)).
+    eapply ptsto_valid; pred_apply; cancel.
+    assert (m acct2 = Some (bal2 ^+ $1)).
+    eapply ptsto_valid; pred_apply; cancel.
+    do 2 combine_opt_eq.
+    simpl; replace (balances s).
+    auto.
+  Qed.
 
   Ltac step :=
     repeat (autounfold with prog);
     eapply pimpl_ok; [ auto with prog | ];
     repeat (autounfold with prog);
     try cancel;
+    try subst;
     eauto.
 
   Ltac hoare := intros; repeat step.
@@ -531,22 +623,7 @@ Section Bank.
   Hint Extern 1 (valid _ _ _ _ (progseq (transfer) _)) => apply transfer_ok : prog.
 
   Definition transfer_yield {T} rx : prog T State :=
-    transfer;; Yield;; rx tt.
-
-  Lemma inv_transfer_stable : forall (bal1 bal2 : valu),
-    #bal1 + #bal2 = 100 ->
-    #bal1 > 0 ->
-    # (bal1 ^- $1) + # (bal2 ^+ $1) = 100.
-  Proof.
-    intros.
-    rewrite wordToNat_minus_one.
-    erewrite wordToNat_plusone.
-    omega.
-    apply lt_wlt.
-    instantiate (1 := $101).
-    simpl; omega.
-    apply gt0_wneq0; auto.
-  Qed.
+    transfer;; Commit record_transfer;; Yield;; rx tt.
 
   Lemma pimpl_and_l : forall AT AEQ V (p q r: @pred AT AEQ V),
     p =p=> r -> p /\ q =p=> r.
@@ -561,28 +638,16 @@ Section Bank.
     {{ F,
       | PRE l: F * inv_rep bal1 bal2 *
            [[ #bal1 > 0 ]] * [[ bankI l #bal1 #bal2 ]]
-      | POST l: RET:_ Inv * [[ bankI l #bal1 #bal2 ]]
+      | POST l': RET:_ Inv * [[ bankI l' (#bal1 - 1) (#bal2 + 1) ]]
     }} transfer_yield.
   Proof.
-    Local Hint Resolve inv_transfer_stable.
+    Hint Resolve inv_transfer_stable.
+    Hint Resolve bank_invariant_transfer.
     unfold transfer_yield.
     intros.
     step.
     step.
-
-    apply pimpl_and_split.
-    cancel.
-    subst.
-    intro; intros.
-    assert (m acct1 = Some (bal1 ^- $1)).
-    eapply ptsto_valid; pred_apply; cancel.
-    assert (m acct2 = Some (bal2 ^+ $1)).
-    eapply ptsto_valid; pred_apply; cancel.
-    rewrite H6 in H0; inversion H0.
-    rewrite H7 in H4; inversion H4.
-    (* this isn't true: the ledger hasn't been correctly updated
-       with a Commit *)
-    admit.
+    step.
 
     (* step'ing over the final continuation calls cancel, which causes
     some evar problems *)
@@ -593,7 +658,11 @@ Section Bank.
     rewrite star_emp_pimpl.
     (* cancel doesn't do this, although it could, if it handled and better *)
     apply pimpl_and_l.
+    (* finish up what step would do *)
     cancel.
-  Abort.
+    subst.
+
+    simpl; replace (balances s); auto.
+  Qed.
 
 End Bank.
